src/ssa/ndopsem_dsop.v
@@ -25,11 +25,7 @@ Require Import ndopsem.
 Export NDopsem.
 Export LLVMopsem.
 
-Definition instantiate_gv (gv:GenericValue) (gvs:GVs) : Prop :=
-match gv with
-| (Vundef, _)::nil => Inhabited _ gvs
-| _ => Same_set _ (Singleton GenericValue gv) gvs
-end.
+Definition instantiate_gv (gv:GenericValue) (gvs:GVs) : Prop := gv @ gvs.
 
 Fixpoint instantiate_locals (lc1 : GVMap) (lc2 : GVsMap) : Prop :=
 match lc1, lc2 with
@@ -108,14 +104,21 @@ Proof.
   unfold Same_set, Included. auto.
 Qed.
 
+Lemma instantiate_undef__undef_gvs : forall m, 
+  instantiate_gv ((Vundef, m) :: nil) (undef_gvs m).
+Proof.
+  intros. unfold undef_gvs.
+  destruct m; apply Union_introl; constructor.
+Qed.
+
 Lemma instantiate_gv__gv2gvs : forall gv, instantiate_gv gv ($ gv $).
 Proof.
   intros.
-  assert (J:=@gv2gvs__inhabited gv).
-  destruct gv; simpl; auto using same_singleton_set.
-    destruct p; simpl.
-    destruct v; simpl; auto using same_singleton_set.     
-    destruct gv; simpl; auto using same_singleton_set.     
+  destruct gv; simpl; try constructor.
+  destruct p; simpl; try constructor.
+  destruct v; simpl; try constructor.
+  destruct gv; simpl; 
+    try solve [constructor | auto using instantiate_undef__undef_gvs].  
 Qed.
 
 Lemma instantiate_locals__getOperandValue : forall TD v lc1 lc2 gl gv1,
@@ -234,16 +237,7 @@ Qed.
 Lemma instantiate_gv__inhabited : forall gv gvs,
   instantiate_gv gv gvs -> Inhabited _ gvs.
 Proof.
-  intros.
-  destruct gv; simpl in *.
-    apply Extensionality_Ensembles in H. subst.
-    apply singleton_inhabited.
-
-    destruct p.
-    destruct v; try solve [auto |
-      apply Extensionality_Ensembles in H; subst; apply singleton_inhabited].
-    destruct gv; try solve [auto |
-      apply Extensionality_Ensembles in H; subst; apply singleton_inhabited].
+  intros. eapply Inhabited_intro; eauto.
 Qed.
 
 Lemma mbop_is_total : forall TD bop0 sz0 x y, 
@@ -259,118 +253,18 @@ Proof.
   destruct bop0; eauto.
 Qed.
 
-Lemma instantiate_gv__mbop__helper : forall x xs y ys TD bop0 sz0
-  (H0 : instantiate_gv x xs)
-  (H1 : instantiate_gv y ys),
-   Inhabited GenericValue
-     (fun gv3 : GenericValue =>
-      exists gv1 : GenericValue,
-        exists gv2 : GenericValue,
-          exists gv3' : GenericValue,
-            gv1 @ xs /\
-            gv2 @ ys /\ mbop TD bop0 sz0 gv1 gv2 = ret gv3' /\ gv3 @ $ gv3' $).
-Proof.
-  intros.
-  apply instantiate_gv__inhabited in H0. inv H0.
-  apply instantiate_gv__inhabited in H1. inv H1.
-  destruct (@mbop_is_total TD bop0 sz0 x0 x1) as [z J].
-  assert (J1:=@gv2gvs__inhabited z). inv J1.
-  exists x2. unfold Ensembles.In. exists x0. exists x1. exists z.
-  split; auto. 
-Qed.
+Hint Unfold instantiate_gv.
 
-Lemma instantiate_gv__mbop : forall TD bop0 sz0 x y z xs ys,
-  mbop TD bop0 sz0 x y = Some z ->
+Lemma instantiate_gv__lift_op2 : forall f x y z xs ys,
+  f x y = Some z ->
   instantiate_gv x xs ->
   instantiate_gv y ys ->
-  instantiate_gv z (lift_op2 (mbop TD bop0 sz0) xs ys).
+  instantiate_gv z (lift_op2 f xs ys).
 Proof.
   intros. unfold lift_op2. 
-  destruct x; try solve [inv H; simpl; 
-      eapply instantiate_gv__mbop__helper; eauto].
-  destruct p.
-  destruct x; try solve [inv H; simpl; 
-      eapply instantiate_gv__mbop__helper; eauto].
-  destruct v; try solve [inv H; simpl; 
-      eapply instantiate_gv__mbop__helper; eauto].
-  destruct y; try solve [inv H; simpl; 
-      eapply instantiate_gv__mbop__helper; eauto].
-  destruct p.
-  destruct y; try solve [inv H; simpl; 
-      eapply instantiate_gv__mbop__helper; eauto].
-  destruct v; try solve [inv H; simpl; 
-      eapply instantiate_gv__mbop__helper; eauto].
-  apply Extensionality_Ensembles in H0. subst.
-  apply Extensionality_Ensembles in H1. subst.
-  assert (J1:=@gv2gvs__inhabited z). inv J1.
-
-  assert (exists v, exists c, z = (v,c)::nil) as EQ.
-    unfold mbop in H.
-    destruct (GV2val TD ((Vint wz i0, m) :: nil));
-      try solve [inv H; unfold gundef; simpl; eauto].
-    destruct v; try solve [inv H; unfold gundef; simpl; eauto].
-    destruct (eq_nat_dec (wz1 + 1) (Size.to_nat sz0));
-      try solve [inv H; unfold gundef; simpl; eauto].
-    destruct (GV2val TD ((Vint wz0 i1, m0) :: nil));
-      try solve [inv H; unfold gundef; simpl; eauto].
-    destruct v; try solve [inv H; unfold gundef; simpl; eauto].
-    unfold val2GV in *.
-    destruct bop0; try solve [inv H; unfold gundef; simpl; eauto].
-    
-  destruct EQ as [v [c EQ]]. subst.
-  simpl.   
-  destruct v.
-    exists x. exists ((Vint wz i0, m) :: nil). exists ((Vint wz0 i1, m0) :: nil).
-    exists ((Vundef, c) :: nil). 
-    repeat (split; try solve [auto | constructor]).
-
-    unfold Same_set, Included.
-    split; intros.
-      inv H1. unfold Ensembles.In. 
-      exists ((Vint wz i0, m) :: nil). exists ((Vint wz0 i1, m0) :: nil).
-      exists ((Vint wz1 i2, c) :: nil). 
-      repeat (split; try solve [auto | constructor]).
-
-      inv H1. unfold Ensembles.In. 
-      destruct H2 as [gv2 [gv3 [J1 [J2 [J3 J4]]]]].
-      inv J1. inv J2.
-      rewrite H in J3. inv J3. inv J4. constructor.
-
-    unfold Same_set, Included.
-    split; intros.
-      inv H1. unfold Ensembles.In. 
-      exists ((Vint wz i0, m) :: nil). exists ((Vint wz0 i1, m0) :: nil).
-      exists ((Vfloat f, c) :: nil). 
-      repeat (split; try solve [auto | constructor]).
-
-      inv H1. unfold Ensembles.In. 
-      destruct H2 as [gv2 [gv3 [J1 [J2 [J3 J4]]]]].
-      inv J1. inv J2.
-      rewrite H in J3. inv J3. inv J4. constructor.
-
-    unfold Same_set, Included.
-    split; intros.
-      inv H0. unfold Ensembles.In. 
-      exists ((Vint wz i0, m) :: nil). exists ((Vint wz0 i1, m0) :: nil).
-      exists ((Vptr b i2, c) :: nil). 
-      repeat (split; try solve [auto | constructor]).
-
-      inv H1. unfold Ensembles.In. 
-      destruct H2 as [gv2 [gv3 [J1 [J2 [J3 J4]]]]].
-      inv J1. inv J2.
-      rewrite H in J3. inv J3. inv J4. constructor.
-
-    unfold Same_set, Included.
-    split; intros.
-      inv H0. unfold Ensembles.In. 
-      exists ((Vint wz i0, m) :: nil). exists ((Vint wz0 i1, m0) :: nil).
-      exists ((Vinttoptr i2, c) :: nil). 
-      repeat (split; try solve [auto | constructor]).
-
-      inv H1. unfold Ensembles.In. 
-      destruct H2 as [gv2 [gv3 [J1 [J2 [J3 J4]]]]].
-      inv J1. inv J2.
-      rewrite H in J3. inv J3. inv J4. constructor.
+  exists x. exists y. exists z. 
+  repeat (split; auto).
+    apply instantiate_gv__gv2gvs.
 Qed.
 
 Lemma instantiate_locals__BOP : forall TD lc1 lc2 gl v1 v2 gv3 bop sz,
@@ -389,7 +283,7 @@ Proof.
   unfold NDopsem.BOP.
   rewrite H1. rewrite H3.
   exists (lift_op2 (mbop TD bop0 sz0) gvs1 gvs2).
-  split; eauto using instantiate_gv__mbop.
+  split; eauto using instantiate_gv__lift_op2.
 Qed.
   
 Lemma mfbop_is_total : forall TD fbop0 fp x y, 
@@ -402,121 +296,6 @@ Proof.
   destruct (GV2val TD y); eauto.
   destruct v; eauto.
   destruct fp; eauto.
-Qed.
-
-Lemma instantiate_gv__mfbop__helper : forall x xs y ys TD fbop0 fp
-  (H0 : instantiate_gv x xs)
-  (H1 : instantiate_gv y ys),
-   Inhabited GenericValue
-     (fun gv3 : GenericValue =>
-      exists gv1 : GenericValue,
-        exists gv2 : GenericValue,
-          exists gv3' : GenericValue,
-            gv1 @ xs /\
-            gv2 @ ys /\ mfbop TD fbop0 fp gv1 gv2 = ret gv3' /\ gv3 @ $ gv3' $).
-Proof.
-  intros.
-  apply instantiate_gv__inhabited in H0. inv H0.
-  apply instantiate_gv__inhabited in H1. inv H1.
-  destruct (@mfbop_is_total TD fbop0 fp x0 x1) as [z J].
-  assert (J1:=@gv2gvs__inhabited z). inv J1.
-  exists x2. unfold Ensembles.In. exists x0. exists x1. exists z.
-  split; auto. 
-Qed.
-
-Lemma instantiate_gv__mfbop : forall TD fbop0 fp x y z xs ys,
-  mfbop TD fbop0 fp x y = Some z ->
-  instantiate_gv x xs ->
-  instantiate_gv y ys ->
-  instantiate_gv z (lift_op2 (mfbop TD fbop0 fp) xs ys).
-Proof.
-  intros. unfold lift_op2.
-  destruct x; try solve [inv H; destruct fp; simpl; 
-      eapply instantiate_gv__mfbop__helper; eauto].
-  destruct p.
-  destruct x; try solve [inv H; destruct fp; simpl; 
-      eapply instantiate_gv__mfbop__helper; eauto].
-  destruct v; try solve [inv H; destruct fp; simpl; 
-      eapply instantiate_gv__mfbop__helper; eauto].
-  destruct y; try solve [inv H; destruct fp; simpl; 
-      eapply instantiate_gv__mfbop__helper; eauto].
-  destruct p.
-  destruct y; try solve [inv H; destruct fp; simpl; 
-      eapply instantiate_gv__mfbop__helper; eauto].
-  destruct v; try solve [inv H; destruct fp; simpl; 
-      eapply instantiate_gv__mfbop__helper; eauto].
-  apply Extensionality_Ensembles in H0. subst.
-  apply Extensionality_Ensembles in H1. subst.
-  assert (J1:=@gv2gvs__inhabited z). inv J1.
-
-  assert (exists v, exists c, z = (v,c)::nil) as EQ.
-    unfold mfbop in H.
-    destruct (GV2val TD ((Vfloat f, m) :: nil));
-      try solve [inv H; destruct fp; unfold gundef, uninits; simpl; eauto].
-    destruct v; try solve 
-      [inv H; destruct fp; unfold gundef, uninits; simpl; eauto].
-    destruct (GV2val TD ((Vfloat f0, m0) :: nil));
-      try solve [inv H; destruct fp; unfold gundef, uninits; simpl; eauto].
-    destruct v; try solve 
-      [inv H; destruct fp; unfold gundef, uninits; simpl; eauto].
-    unfold val2GV in *.
-    destruct fp; destruct fbop0; 
-      try solve [inv H; unfold gundef, uninits; simpl; eauto].
-    
-  destruct EQ as [v [c EQ]]. subst.
-  simpl.   
-  destruct v.
-    exists x. exists ((Vfloat f, m) :: nil). exists ((Vfloat f0, m0) :: nil).
-    exists ((Vundef, c) :: nil). 
-    repeat (split; try solve [auto | constructor]).
-
-    unfold Same_set, Included.
-    split; intros.
-      inv H1. unfold Ensembles.In. 
-      exists ((Vfloat f, m) :: nil). exists ((Vfloat f0, m0) :: nil).
-      exists ((Vint wz i0, c) :: nil). 
-      repeat (split; try solve [auto | constructor]).
-
-      inv H1. unfold Ensembles.In. 
-      destruct H2 as [gv2 [gv3 [J1 [J2 [J3 J4]]]]].
-      inv J1. inv J2.
-      rewrite H in J3. inv J3. inv J4. constructor.
-
-    unfold Same_set, Included.
-    split; intros.
-      inv H1. unfold Ensembles.In. 
-      exists ((Vfloat f, m) :: nil). exists ((Vfloat f0, m0) :: nil).
-      exists ((Vfloat f1, c) :: nil). 
-      repeat (split; try solve [auto | constructor]).
-
-      inv H1. unfold Ensembles.In. 
-      destruct H2 as [gv2 [gv3 [J1 [J2 [J3 J4]]]]].
-      inv J1. inv J2.
-      rewrite H in J3. inv J3. inv J4. constructor.
-
-    unfold Same_set, Included.
-    split; intros.
-      inv H0. unfold Ensembles.In. 
-      exists ((Vfloat f, m) :: nil). exists ((Vfloat f0, m0) :: nil).
-      exists ((Vptr b i0, c) :: nil). 
-      repeat (split; try solve [auto | constructor]).
-
-      inv H1. unfold Ensembles.In. 
-      destruct H2 as [gv2 [gv3 [J1 [J2 [J3 J4]]]]].
-      inv J1. inv J2.
-      rewrite H in J3. inv J3. inv J4. constructor.
-
-    unfold Same_set, Included.
-    split; intros.
-      inv H0. unfold Ensembles.In. 
-      exists ((Vfloat f, m) :: nil). exists ((Vfloat f0, m0) :: nil).
-      exists ((Vinttoptr i0, c) :: nil). 
-      repeat (split; try solve [auto | constructor]).
-
-      inv H1. unfold Ensembles.In. 
-      destruct H2 as [gv2 [gv3 [J1 [J2 [J3 J4]]]]].
-      inv J1. inv J2.
-      rewrite H in J3. inv J3. inv J4. constructor.
 Qed.
 
 Lemma instantiate_locals__FBOP : forall TD lc1 lc2 gl v1 v2 gv3 fbop fp,
@@ -535,7 +314,7 @@ Proof.
   unfold NDopsem.FBOP.
   rewrite H1. rewrite H3.
   exists (lift_op2 (mfbop TD fbop0 fp) gvs1 gvs2).
-  split; eauto using instantiate_gv__mfbop.
+  split; eauto using instantiate_gv__lift_op2.
 Qed.
 
 Lemma micmp_is_total : forall TD c t x y, 
@@ -549,122 +328,6 @@ Proof.
   destruct (GV2val TD y); eauto.
   destruct v; eauto.
   destruct c; eauto.
-Qed.
-
-Lemma instantiate_gv__micmp__helper : forall x xs y ys TD c t
-  (H0 : instantiate_gv x xs)
-  (H1 : instantiate_gv y ys),
-   Inhabited GenericValue
-     (fun gv3 : GenericValue =>
-      exists gv1 : GenericValue,
-        exists gv2 : GenericValue,
-          exists gv3' : GenericValue,
-            gv1 @ xs /\
-            gv2 @ ys /\ micmp TD c t gv1 gv2 = ret gv3' /\ gv3 @ $ gv3' $).
-Proof.
-  intros.
-  apply instantiate_gv__inhabited in H0. inv H0.
-  apply instantiate_gv__inhabited in H1. inv H1.
-  destruct (@micmp_is_total TD c t x0 x1) as [z J].
-  assert (J1:=@gv2gvs__inhabited z). inv J1.
-  exists x2. unfold Ensembles.In. exists x0. exists x1. exists z.
-  split; auto. 
-Qed.
-
-Lemma instantiate_gv__micmp : forall TD c t x y z xs ys,
-  micmp TD c t x y = Some z ->
-  instantiate_gv x xs ->
-  instantiate_gv y ys ->
-  instantiate_gv z (lift_op2 (micmp TD c t) xs ys).
-Proof.
-  intros. unfold lift_op2.
-  unfold micmp in H.
-Opaque micmp.
-  destruct t; try solve [inv H; simpl; 
-      eapply instantiate_gv__micmp__helper; eauto].
-  destruct x; try solve [inv H; simpl; 
-      eapply instantiate_gv__micmp__helper; eauto].
-  destruct p.
-  destruct x; try solve [inv H; simpl; 
-      eapply instantiate_gv__micmp__helper; eauto].
-  destruct v; try solve [inv H; simpl; 
-      eapply instantiate_gv__micmp__helper; eauto].
-  destruct y; try solve [inv H; simpl; 
-      eapply instantiate_gv__micmp__helper; eauto].
-  destruct p.
-  destruct y; try solve [inv H; simpl; 
-      eapply instantiate_gv__micmp__helper; eauto].
-  destruct v; try solve [inv H; simpl; 
-      eapply instantiate_gv__micmp__helper; eauto].
-  apply Extensionality_Ensembles in H0. subst.
-  apply Extensionality_Ensembles in H1. subst.
-  assert (J1:=@gv2gvs__inhabited z). inv J1.
-Transparent micmp.
-  assert (exists v, exists c, z = (v,c)::nil) as EQ.
-    unfold micmp_int in H.
-    destruct (GV2val TD ((Vint wz i0, m) :: nil));
-      try solve [inv H; unfold gundef; simpl; eauto].
-    destruct v; try solve [inv H; unfold gundef; simpl; eauto].
-    destruct (GV2val TD ((Vint wz0 i1, m0) :: nil));
-      try solve [inv H; unfold gundef; simpl; eauto].
-    destruct v; try solve [inv H; unfold gundef; simpl; eauto].
-    unfold val2GV in *.
-    destruct c; try solve [inv H; unfold gundef; simpl; eauto].
-    
-  destruct EQ as [v [c' EQ]]. subst.
-  simpl.   
-  destruct v.
-    exists x. exists ((Vint wz i0, m) :: nil). exists ((Vint wz0 i1, m0) :: nil).
-    exists ((Vundef, c') :: nil). 
-    repeat (split; try solve [auto | constructor]).
-
-    unfold Same_set, Included.
-    split; intros.
-      inv H1. unfold Ensembles.In.
-      exists ((Vint wz i0, m) :: nil). exists ((Vint wz0 i1, m0) :: nil). 
-      exists ((Vint wz1 i2, c') :: nil). 
-      repeat (split; try solve [auto | constructor]).
-
-      inv H1. unfold Ensembles.In. 
-      destruct H2 as [gv2 [gv3 [J1 [J2 [J3 J4]]]]].
-      inv J1. inv J2.
-      rewrite H in J3. inv J3. inv J4. constructor.
-
-    unfold Same_set, Included.
-    split; intros.
-      inv H1. unfold Ensembles.In. 
-      exists ((Vint wz i0, m) :: nil). exists ((Vint wz0 i1, m0) :: nil). 
-      exists ((Vfloat f, c') :: nil). 
-      repeat (split; try solve [auto | constructor]).
-
-      inv H1. unfold Ensembles.In. 
-      destruct H2 as [gv2 [gv3 [J1 [J2 [J3 J4]]]]].
-      inv J1. inv J2.
-      rewrite H in J3. inv J3. inv J4. constructor.
-
-    unfold Same_set, Included.
-    split; intros.
-      inv H0. unfold Ensembles.In. 
-      exists ((Vint wz i0, m) :: nil). exists ((Vint wz0 i1, m0) :: nil). 
-      exists ((Vptr b i2, c') :: nil). 
-      repeat (split; try solve [auto | constructor]).
-
-      inv H1. unfold Ensembles.In. 
-      destruct H2 as [gv2 [gv3 [J1 [J2 [J3 J4]]]]].
-      inv J1. inv J2.
-      rewrite H in J3. inv J3. inv J4. constructor.
-
-    unfold Same_set, Included.
-    split; intros.
-      inv H0. unfold Ensembles.In. 
-      exists ((Vint wz i0, m) :: nil). exists ((Vint wz0 i1, m0) :: nil). 
-      exists ((Vinttoptr i2, c') :: nil). 
-      repeat (split; try solve [auto | constructor]).
-
-      inv H1. unfold Ensembles.In. 
-      destruct H2 as [gv2 [gv3 [J1 [J2 [J3 J4]]]]].
-      inv J1. inv J2.
-      rewrite H in J3. inv J3. inv J4. constructor.
 Qed.
 
 Lemma instantiate_locals__ICMP : forall TD lc1 lc2 gl v1 v2 gv3 c t,
@@ -683,7 +346,7 @@ Proof.
   unfold NDopsem.ICMP.
   rewrite H1. rewrite H3.
   exists (lift_op2 (micmp TD c t) gvs1 gvs2).
-  split; eauto using instantiate_gv__micmp.
+  split; eauto using instantiate_gv__lift_op2.
 Qed.
 
 Lemma mfcmp_is_total : forall TD c t x y, 
@@ -696,114 +359,6 @@ Proof.
   destruct (GV2val TD y); eauto.
   destruct v; eauto.
   destruct t; destruct c; eauto.
-Qed.
-
-Lemma instantiate_gv__mfcmp__helper : forall x xs y ys TD c t
-  (H0 : instantiate_gv x xs)
-  (H1 : instantiate_gv y ys),
-   Inhabited GenericValue
-     (fun gv3 : GenericValue =>
-      exists gv1 : GenericValue,
-        exists gv2 : GenericValue,
-          exists gv3' : GenericValue,
-            gv1 @ xs /\
-            gv2 @ ys /\ mfcmp TD c t gv1 gv2 = ret gv3' /\ gv3 @ $ gv3' $).
-Proof.
-  intros.
-  apply instantiate_gv__inhabited in H0. inv H0.
-  apply instantiate_gv__inhabited in H1. inv H1.
-  destruct (@mfcmp_is_total TD c t x0 x1) as [z J].
-  assert (J1:=@gv2gvs__inhabited z). inv J1.
-  exists x2. unfold Ensembles.In. exists x0. exists x1. exists z.
-  split; auto. 
-Qed.
-
-Lemma instantiate_gv__mfcmp : forall TD c t x y z xs ys,
-  mfcmp TD c t x y = Some z ->
-  instantiate_gv x xs ->
-  instantiate_gv y ys ->
-  instantiate_gv z (lift_op2 (mfcmp TD c t) xs ys).
-Proof.
-  intros. unfold lift_op2.
-  unfold mfcmp in H.
-Opaque mfcmp.
-  destruct x; try solve [inv H; simpl; 
-      eapply instantiate_gv__mfcmp__helper; eauto].
-  destruct p.
-  destruct x; try solve [inv H; simpl; 
-      eapply instantiate_gv__mfcmp__helper; eauto].
-  destruct v; try solve [inv H; simpl; 
-      eapply instantiate_gv__mfcmp__helper; eauto].
-  destruct y; try solve [inv H; simpl; 
-      eapply instantiate_gv__mfcmp__helper; eauto].
-  destruct p.
-  destruct y; try solve [inv H; simpl; 
-      eapply instantiate_gv__mfcmp__helper; eauto].
-  destruct v; try solve [inv H; simpl; 
-      eapply instantiate_gv__mfcmp__helper; eauto].
-  simpl in H.
-  apply Extensionality_Ensembles in H0. subst.
-  apply Extensionality_Ensembles in H1. subst.
-  assert (J1:=@gv2gvs__inhabited z). inv J1.
-Transparent mfcmp.
-  assert (exists v, exists c, z = (v,c)::nil) as EQ.
-    unfold val2GV in *.
-    destruct t; destruct c; try solve [inv H; unfold gundef; simpl; eauto].
-  destruct EQ as [v [c' EQ]]. subst.
-  unfold mfcmp.
-  simpl.   
-  destruct v.
-    exists x. exists ((Vfloat f, m) :: nil). exists ((Vfloat f0, m0) :: nil).
-    exists ((Vundef, c') :: nil). 
-    repeat (split; try solve [auto | constructor]).
-
-    unfold Same_set, Included.
-    split; intros.
-      inv H1. unfold Ensembles.In.
-      exists ((Vfloat f, m) :: nil). exists ((Vfloat f0, m0) :: nil).
-      exists ((Vint wz i0, c') :: nil). 
-      repeat (split; try solve [auto | constructor]).
-
-      inv H1. unfold Ensembles.In. 
-      destruct H2 as [gv2 [gv3 [J1 [J2 [J3 J4]]]]].
-      inv J1. inv J2. simpl in J3.
-      rewrite H in J3. inv J3. inv J4. constructor.
-
-    unfold Same_set, Included.
-    split; intros.
-      inv H1. unfold Ensembles.In. 
-      exists ((Vfloat f, m) :: nil). exists ((Vfloat f0, m0) :: nil).
-      exists ((Vfloat f1, c') :: nil). 
-      repeat (split; try solve [auto | constructor]).
-
-      inv H1. unfold Ensembles.In. 
-      destruct H2 as [gv2 [gv3 [J1 [J2 [J3 J4]]]]].
-      inv J1. inv J2. simpl in J3.
-      rewrite H in J3. inv J3. inv J4. constructor.
-
-    unfold Same_set, Included.
-    split; intros.
-      inv H0. unfold Ensembles.In. 
-      exists ((Vfloat f, m) :: nil). exists ((Vfloat f0, m0) :: nil).
-      exists ((Vptr b i0, c') :: nil). 
-      repeat (split; try solve [auto | constructor]).
-
-      inv H1. unfold Ensembles.In. 
-      destruct H2 as [gv2 [gv3 [J1 [J2 [J3 J4]]]]].
-      inv J1. inv J2. simpl in J3.
-      rewrite H in J3. inv J3. inv J4. constructor.
-
-    unfold Same_set, Included.
-    split; intros.
-      inv H0. unfold Ensembles.In. 
-      exists ((Vfloat f, m) :: nil). exists ((Vfloat f0, m0) :: nil).
-      exists ((Vinttoptr i0, c') :: nil). 
-      repeat (split; try solve [auto | constructor]).
-
-      inv H1. unfold Ensembles.In. 
-      destruct H2 as [gv2 [gv3 [J1 [J2 [J3 J4]]]]].
-      inv J1. inv J2. simpl in J3.
-      rewrite H in J3. inv J3. inv J4. constructor.
 Qed.
 
 Lemma instantiate_locals__FCMP : forall TD lc1 lc2 gl v1 v2 gv3 c t,
@@ -822,7 +377,7 @@ Proof.
   unfold NDopsem.FCMP.
   rewrite H1. rewrite H3.
   exists (lift_op2 (mfcmp TD c t) gvs1 gvs2).
-  split; eauto using instantiate_gv__mfcmp.
+  split; eauto using instantiate_gv__lift_op2.
 Qed.
 
 Fixpoint instantiate_gvs (l1 : list GenericValue) (l2 : list GVs) :=
@@ -875,7 +430,7 @@ Proof.
   destruct ptr; inv H.
   simpl. congruence.
 Qed.
-
+(*
 Lemma defined_gv__instantiate_gv : forall gv gvs,
   defined_gv gv -> instantiate_gv gv gvs -> gv @ gvs.
 Proof.
@@ -975,7 +530,7 @@ Proof.
     inv H. eapply IHgv1 in H2; eauto.
     subst. auto.
 Qed.
-
+*)
 Lemma GEP_is_total : forall TD t mp vidxs inbounds0,
   exists mp', LLVMgv.GEP TD t mp vidxs inbounds0 = ret mp'.
 Proof.
@@ -998,7 +553,7 @@ Proof.
     inv H0.
     exists (x::gv1). simpl. auto.
 Qed.    
-
+(*
 Lemma instantiate_locals__GEP_helper : forall vidxs vidxss mp1 mps2 TD t
   inbounds (Hinst1 : instantiate_gvs vidxs vidxss)
   (Hinst2 : instantiate_gv mp1 mps2),
@@ -1018,7 +573,7 @@ Proof.
   exists x0. unfold Ensembles.In. exists x. exists gv1. exists gv2.
   split; auto. 
 Qed.  
-
+*)
 Lemma instantiate_locals__GEP : forall TD t mp1 mp1' vidxs vidxss inbounds mps2,
   instantiate_gvs vidxs vidxss ->
   instantiate_gv mp1 mps2 ->
@@ -1029,57 +584,17 @@ Proof.
   intros TD t mp1 mp1' vidxs vidxss inbounds mps2 Hinst1 Hinst2 Hgep.
   unfold NDopsem.GEP.
   exists (fun gv : GenericValue =>
-        exists ma : GenericValue,
-          exists vidxs0 : list GenericValue,
-            exists gv' : GenericValue,
-              ma @ mps2 /\
-              vidxs0 @@ vidxss /\
-              GEP TD t ma vidxs0 inbounds = ret gv' /\ gv @ $ gv' $).
-  split; auto. 
-  unfold GEP in Hgep.
-  remember (GV2ptr TD (getPointerSize TD) mp1) as R.
-  destruct R; try solve [inv Hgep; simpl; 
-      eapply instantiate_locals__GEP_helper; eauto].
-  remember (GVs2Nats TD vidxs) as R1.
-  destruct R1; try solve [inv Hgep; simpl; 
-      eapply instantiate_locals__GEP_helper; eauto].
-  remember (mgep TD t v l0) as R2.
-  destruct R2; try solve [inv Hgep; simpl; 
-      eapply instantiate_locals__GEP_helper; eauto].
-  inv Hgep. 
-  unfold mgep in HeqR2.
-  destruct v; tinv HeqR2.
-  destruct l0; tinv HeqR2.
-  remember (mgetoffset TD (typ_array 0%nat t) (z :: l0)) as R3.
-  destruct R3 as [[o ?]|]; inv HeqR2.
-  unfold ptr2GV, val2GV. simpl.
-  symmetry in HeqR.
-  assert (J:=HeqR).
-  apply GV2ptr__defined_gv in J. 
-  apply defined_gv__same_singleton in Hinst2; auto. subst.
-  symmetry in HeqR1.
-  assert (J1:=HeqR1).
-  apply GVs2Nats__defined_gvs in J1. 
-  assert (J9:=Hinst1).
-  apply defined_gvs__instantiate_gvs in J9; auto. 
-  apply defined_gvs__same_singleton in Hinst1; auto. 
-  unfold Same_set, Included.
-  split; intros.
-    inv H. unfold Ensembles.In.
-    exists mp1.
-    exists vidxs. 
-    exists ((Vptr b (Int.add 31 i0 o), AST.Mint (getPointerSize TD - 1)) :: nil).
+          exists ma : GenericValue,
+            exists vidxs0 : list GenericValue,
+              exists gv' : GenericValue,
+                ma @ mps2 /\
+                vidxs0 @@ vidxss /\
+                GEP TD t ma vidxs0 inbounds = ret gv' /\ gv @ $ gv' $).
+  split; auto.
+    unfold instantiate_gv, Ensembles.In.
+    exists mp1. exists vidxs. exists mp1'.
     repeat (split; auto).
-    unfold GEP. rewrite HeqR. rewrite HeqR1. unfold mgep.
-    rewrite <- HeqR3. unfold ptr2GV, val2GV. auto.
-
-    inv H. destruct H0 as [A [B [J1' [J2 [J3 J4]]]]].
-    eapply singletons_spec in Hinst1; eauto. subst.
-    inv J1'. unfold GEP in J3.
-    rewrite HeqR in J3. rewrite HeqR1 in J3. unfold mgep in J3.
-    rewrite <- HeqR3 in J3. inv J3. inv J4.
-    unfold ptr2GV, val2GV. 
-    unfold Ensembles.In. constructor.
+      apply instantiate_gv__gv2gvs.
 Qed.
 
 Lemma mget'_is_total : forall TD ofs t' x, 
@@ -1092,22 +607,6 @@ Proof.
   destruct p.  
   destruct (splitGenericValue g0 (Z_of_nat n)); eauto.
   destruct p. eauto.
-Qed.
-
-Lemma instantiate_gv__mget'__helper : forall x xs TD ofs t'
-  (H0 : instantiate_gv x xs),
-   Inhabited GenericValue
-     (fun gv2 : GenericValue =>
-      exists gv1 : GenericValue,
-        exists gv2' : GenericValue,
-          gv1 @ xs /\ mget' TD ofs t' gv1 = ret gv2' /\ gv2 @ $ gv2' $).
-Proof.
-  intros.
-  apply instantiate_gv__inhabited in H0. inv H0.
-  destruct (@mget'_is_total TD ofs t' x0) as [z J].
-  assert (J1:=@gv2gvs__inhabited z). inv J1.
-  exists x1. unfold Ensembles.In. exists x0. exists z.
-  split; auto. 
 Qed.
 
 Lemma defined_gv__spec1 : forall gv,
@@ -1133,131 +632,22 @@ Proof.
     ].
 Qed.      
 
-Lemma instantiate_gv__mget'__helper2 : forall TD ofs t' x gv,
-  mget' TD ofs t' x = ret gv ->
-  defined_gv gv ->
-   Same_set GenericValue (Singleton GenericValue gv)
-     (fun gv2 : GenericValue =>
-      exists gv1 : GenericValue, exists gv2' : GenericValue,
-        gv1 @ Singleton GenericValue x /\
-        mget' TD ofs t' gv1 = ret gv2' /\ gv2 @ $ gv2' $).
-Proof.
-  intros.
-    unfold Same_set, Included.    
-    split; intros.
-      inv H1. unfold Ensembles.In. exists x. exists x0.
-      split; auto. constructor. split; auto. apply defined_gv__spec1; auto.
-
-      inv H1. destruct H2 as [A [J1 [J2 J3]]].
-      inv J1. rewrite J2 in H. inv H. 
-      apply defined_gv__spec2 in H0. rewrite H0 in J3. inv J3. 
-      unfold Ensembles.In. constructor.
-Qed.  
-
-Lemma instantiate_gv__mget'__helper3 : forall TD ofs t' x z xs n
-  (HeqR : ret n = getTypeStoreSize TD t')
-  (g : GenericValue)
-  (gvr : GenericValue)
-  (HeqR1 : ret (g, gvr) = splitGenericValue x (Int.signed 31 ofs))
-  (gvrl : GenericValue)
-  (H0 : Same_set _ (Singleton _ x) xs)
-  (HeqR2 : ret (z, gvrl) = splitGenericValue gvr (Z_of_nat n)),
-   instantiate_gv z
-     (fun gv2 : GenericValue =>
-      exists gv1 : GenericValue, exists gv2' : GenericValue,
-        gv1 @ xs /\ mget' TD ofs t' gv1 = ret gv2' /\ gv2 @ $ gv2'$).
-Proof.
-  intros.
-  assert (mget' TD ofs t' x = ret z) as J.
-    unfold mget'. unfold mget.
-    rewrite <- HeqR. simpl.
-    rewrite <- HeqR1. rewrite <- HeqR2. split; auto. 
-  apply Extensionality_Ensembles in H0. subst. 
-  assert (J1:=@gv2gvs__inhabited z). inv J1.
-  destruct z; simpl.
-    eapply instantiate_gv__mget'__helper2; simpl; eauto.
-
-    destruct p.
-    destruct v.
-      destruct z.
-        exists x0. unfold Ensembles.In. exists x. exists ((Vundef, m) :: nil).
-        split. constructor. split; auto.
-
-        simpl in H. inv H.
-        unfold Same_set, Included.    
-        split; intros.
-          inv H. unfold Ensembles.In. exists x. exists ((Vundef, m) :: p :: z).
-          split. constructor. simpl. split; auto. constructor.
-
-          inv H. destruct H0 as [A [J1 [J2 J3]]].
-          inv J1. rewrite J2 in J. inv J. inv J3.  constructor.
-      eapply instantiate_gv__mget'__helper2; simpl; 
-        try solve [eauto | congruence].
-      eapply instantiate_gv__mget'__helper2; simpl; 
-        try solve [eauto | congruence].
-      eapply instantiate_gv__mget'__helper2; simpl; 
-        try solve [eauto | congruence].
-      eapply instantiate_gv__mget'__helper2; simpl; 
-        try solve [eauto | congruence].
-Qed.
-
-Lemma instantiate_gv__mget' : forall TD ofs t' x z xs,
-  mget' TD ofs t' x = Some z ->
-  defined_gv x ->
+Lemma instantiate_gv__lift_op1 : forall f x z xs,
+  f x = Some z ->
   instantiate_gv x xs ->
-  instantiate_gv z (lift_op1 (mget' TD ofs t') xs).
+  instantiate_gv z (lift_op1 f xs).
 Proof.
-  intros TD ofs t' x z xs H G H0. unfold lift_op1. 
-  unfold mget', mget in H.
-Opaque mget'. 
-  remember (getTypeStoreSize TD t') as R.
-  destruct R; try solve [
-    destruct t'; try solve [
-      inv H; simpl; eapply instantiate_gv__mget'__helper; eauto |
-      destruct f; try solve [inv H; simpl; 
-        eapply instantiate_gv__mget'__helper; eauto]
-    ]
-  ].
-  simpl in H.
-  remember (splitGenericValue x (Int.signed 31 ofs)) as R1.
-  destruct R1 as [[? gvr]|]; try solve [
-    destruct t'; try solve [
-      inv H; simpl; eapply instantiate_gv__mget'__helper; eauto |
-      destruct f; try solve [inv H; simpl; 
-        eapply instantiate_gv__mget'__helper; eauto]
-    ]
-  ].
-  remember (splitGenericValue gvr (Z_of_nat n)) as R2.
-  destruct R2 as [[? gvrl]|]; try solve [
-    destruct t'; try solve [
-      inv H; simpl; eapply instantiate_gv__mget'__helper; eauto |
-      destruct f; try solve [inv H; simpl; 
-        eapply instantiate_gv__mget'__helper; eauto]
-    ]
-  ].
-  inv H. 
-
-  destruct x.
-    eapply instantiate_gv__mget'__helper3; eauto.
-    destruct p.
-    destruct v.
-      destruct x.      
-        simpl in G. contradict G; auto.
-        eapply instantiate_gv__mget'__helper3; eauto.
-      eapply instantiate_gv__mget'__helper3; eauto.
-      eapply instantiate_gv__mget'__helper3; eauto.
-      eapply instantiate_gv__mget'__helper3; eauto.
-      eapply instantiate_gv__mget'__helper3; eauto.
-
-Transparent mget'. 
-Qed.    
+  intros. unfold lift_op1. 
+  exists x. exists z. 
+  repeat (split; auto).
+    apply instantiate_gv__gv2gvs.
+Qed.
 
 Lemma instantiate_locals__extractGenericValue : forall TD lc1 lc2 t gv2
     cidxs gv1 gvs1,
   instantiate_locals lc1 lc2 -> 
   instantiate_gv gv1 gvs1 ->
   extractGenericValue TD t gv1 cidxs = Some gv2 ->
-  defined_gv gv1 ->
   exists gvs2, NDopsem.extractGenericValue TD t gvs1 cidxs = Some gvs2 
     /\ instantiate_gv gv2 gvs2.
 Proof.
@@ -1265,10 +655,10 @@ Proof.
   unfold extractGenericValue in H1.
   unfold NDopsem.extractGenericValue.
   destruct (intConsts2Nats TD cidxs); inv H1.
-    destruct (mgetoffset TD t l0) as [[]|]; inv H4.
+    destruct (mgetoffset TD t l0) as [[]|]; inv H3.
       exists (lift_op1 (mget' TD i0 t0) gvs1).
       split; auto.
-        eapply instantiate_gv__mget'; eauto.
+        eapply instantiate_gv__lift_op1; eauto.
       exists ($ uninits 1 $). split; auto using instantiate_gv__gv2gvs.
     exists ($ uninits 1 $). split; auto using instantiate_gv__gv2gvs.
 Qed.
@@ -1282,153 +672,12 @@ Proof.
   destruct (mset TD x ofs t2 y); eauto.
 Qed.  
 
-Lemma instantiate_gv__mset'__helper : forall x xs y ys TD ofs t1 t2
-  (H0 : instantiate_gv x xs) (H1 : instantiate_gv y ys),
-   Inhabited GenericValue
-     (fun gv3 : GenericValue =>
-      exists gv1 : GenericValue, exists gv2 : GenericValue,
-        exists gv3' : GenericValue,
-          gv1 @ xs /\ gv2 @ ys /\ 
-          mset' TD ofs t1 t2 gv1 gv2 = ret gv3' /\ gv3 @ $ gv3' $).
-Proof.
-  intros.
-  apply instantiate_gv__inhabited in H0. inv H0.
-  apply instantiate_gv__inhabited in H1. inv H1.
-  destruct (@mset'_is_total TD ofs t1 t2 x0 x1) as [z J].
-  assert (J1:=@gv2gvs__inhabited z). inv J1.
-  exists x2. unfold Ensembles.In. exists x0. exists x1. exists z.
-  repeat (split; auto). 
-Qed.
-
-Lemma instantiate_gv__mset' : forall TD ofs t1 t2 x y z xs ys,
-  mset' TD ofs t1 t2 x y = Some z ->
-  defined_gv x ->
-  defined_gv y ->
-  instantiate_gv x xs ->
-  instantiate_gv y ys ->
-  instantiate_gv z (lift_op2 (mset' TD ofs t1 t2) xs ys).
-Proof.
-  intros TD ofs t1 t2 x y z xs ys H G G' H0 H1. unfold lift_op2. 
-  unfold mset', mset in H.
-Opaque mset'. 
-  remember (getTypeStoreSize TD t2) as R.
-  destruct R; try solve [
-    destruct t1; try solve [
-      inv H; simpl; eapply instantiate_gv__mset'__helper; eauto |
-      destruct f; try solve [inv H; simpl; 
-        eapply instantiate_gv__mset'__helper; eauto]
-    ]
-  ].
-  simpl in H.
-  remember (n =n= length y) as R0.
-  destruct R0; try solve [
-    destruct t1; try solve [
-      inv H; simpl; eapply instantiate_gv__mset'__helper; eauto |
-      destruct f; try solve [inv H; simpl; 
-        eapply instantiate_gv__mset'__helper; eauto]
-    ]
-  ].
-  remember (splitGenericValue x (Int.signed 31 ofs)) as R1.
-  destruct R1 as [[? gvr]|]; try solve [
-    destruct t1; try solve [
-      inv H; simpl; eapply instantiate_gv__mset'__helper; eauto |
-      destruct f; try solve [inv H; simpl; 
-        eapply instantiate_gv__mset'__helper; eauto]
-    ]
-  ].
-  remember (splitGenericValue gvr (Z_of_nat n)) as R2.
-  destruct R2 as [[? gvrl]|]; try solve [
-    destruct t1; try solve [
-      inv H; simpl; eapply instantiate_gv__mset'__helper; eauto |
-      destruct f; try solve [inv H; simpl; 
-        eapply instantiate_gv__mset'__helper; eauto]
-    ]
-  ].
-  inv H. 
-  apply defined_gv__same_singleton in H0; auto. subst.
-  apply defined_gv__same_singleton in H1; auto. subst.
-Transparent mset'. 
- 
-  assert (mset' TD ofs t1 t2 x y = Some (g ++ y ++ gvrl)) as J.
-    unfold mset', mset.
-    rewrite <- HeqR. simpl. rewrite <- HeqR0. rewrite <- HeqR1. rewrite <- HeqR2.
-    auto.
-  assert (J1:=@gv2gvs__inhabited (g ++ y ++ gvrl)). inv J1.
-  destruct (g ++ y ++ gvrl).
-    simpl. unfold Same_set, Included.
-    inv H.
-    split; intros.
-      inv H. unfold Ensembles.In. exists x. exists y. exists nil. simpl.
-      split. constructor. split. constructor. split; auto. constructor.
-
-      inv H. destruct H0 as [A [B [J1 [J2 [J3 J4]]]]]. inv J1. inv J2. 
-      rewrite J3 in J. inv J. inv J4. unfold Ensembles.In. constructor.
-    destruct p.
-    destruct v.
-      destruct l0.
-        simpl. exists x0. unfold Ensembles.In. exists x. exists y.
-        exists ((Vundef, m) :: nil). split. constructor. split. constructor.
-        split; auto.
-
-    simpl. unfold Same_set, Included.
-    inv H.
-    split; intros.
-      inv H. unfold Ensembles.In. exists x. exists y. 
-      exists ((Vundef, m) :: p :: l0). simpl.
-      split. constructor. split. constructor. split; auto. constructor.
-
-      inv H. destruct H0 as [A [B [J1 [J2 [J3 J4]]]]]. inv J1. inv J2. 
-      rewrite J3 in J. inv J. inv J4. unfold Ensembles.In. constructor.
-
-    simpl. unfold Same_set, Included.
-    inv H.
-    split; intros.
-      inv H. unfold Ensembles.In. exists x. exists y. 
-      exists ((Vint wz i0, m) :: l0). simpl.
-      split. constructor. split. constructor. split; auto. constructor.
-
-      inv H. destruct H0 as [A [B [J1 [J2 [J3 J4]]]]]. inv J1. inv J2. 
-      rewrite J3 in J. inv J. inv J4. unfold Ensembles.In. constructor.
-
-    simpl. unfold Same_set, Included.
-    inv H.
-    split; intros.
-      inv H. unfold Ensembles.In. exists x. exists y. 
-      exists ((Vfloat f, m) :: l0). simpl.
-      split. constructor. split. constructor. split; auto. constructor.
-
-      inv H. destruct H0 as [A [B [J1 [J2 [J3 J4]]]]]. inv J1. inv J2. 
-      rewrite J3 in J. inv J. inv J4. unfold Ensembles.In. constructor.
-
-    simpl. unfold Same_set, Included.
-    inv H.
-    split; intros.
-      inv H. unfold Ensembles.In. exists x. exists y. 
-      exists ((Vptr b i0, m) :: l0). simpl.
-      split. constructor. split. constructor. split; auto. constructor.
-
-      inv H. destruct H0 as [A [B [J1 [J2 [J3 J4]]]]]. inv J1. inv J2. 
-      rewrite J3 in J. inv J. inv J4. unfold Ensembles.In. constructor.
-
-    simpl. unfold Same_set, Included.
-    inv H.
-    split; intros.
-      inv H. unfold Ensembles.In. exists x. exists y. 
-      exists ((Vinttoptr i0, m) :: l0). simpl.
-      split. constructor. split. constructor. split; auto. constructor.
-
-      inv H. destruct H0 as [A [B [J1 [J2 [J3 J4]]]]]. inv J1. inv J2. 
-      rewrite J3 in J. inv J. inv J4. unfold Ensembles.In. constructor.
-Qed.    
-
 Lemma instantiate_locals__insertGenericValue : forall TD lc1 lc2 t1 t2 gv2 
     cidxs gv1 gvs1 gvs2 gv3,
   instantiate_locals lc1 lc2 -> 
   instantiate_gv gv1 gvs1 ->
   instantiate_gv gv2 gvs2 ->
   insertGenericValue TD t1 gv1 cidxs t2 gv2 = Some gv3 ->
-  defined_gv gv1 ->
-  defined_gv gv2 ->
   exists gvs3, NDopsem.insertGenericValue TD t1 gvs1 cidxs t2 gvs2 = Some gvs3
     /\ instantiate_gv gv3 gvs3.
 Proof.
@@ -1436,10 +685,10 @@ Proof.
   unfold insertGenericValue in H2.
   unfold NDopsem.insertGenericValue.
   destruct (intConsts2Nats TD cidxs); inv H2.
-    destruct (mgetoffset TD t1 l0) as [[]|]; inv H6.
+    destruct (mgetoffset TD t1 l0) as [[]|]; inv H4.
       exists (lift_op2 (mset' TD i0 t1 t2) gvs1 gvs2).
       split; auto.
-        eapply instantiate_gv__mset'; eauto.
+        eapply instantiate_gv__lift_op2; eauto.
       exists ($ gundef t1 $). split; auto using instantiate_gv__gv2gvs.
     exists ($ gundef t1 $). split; auto using instantiate_gv__gv2gvs.
 Qed.
@@ -1451,131 +700,6 @@ Proof.
   unfold mcast, mbitcast.
   destruct cop0; destruct t1; destruct t2; eauto.
 Qed.
-
-Lemma instantiate_gv__mcast__helper : forall x xs TD op t1 t2
-  (H0 : instantiate_gv x xs),
-   Inhabited GenericValue
-     (fun gv2 : GenericValue =>
-      exists gv1 : GenericValue,
-        exists gv2' : GenericValue,
-            gv1 @ xs /\ mcast TD op t1 t2 gv1 = ret gv2' /\ gv2 @ $ gv2' $).
-Proof.
-  intros.
-  apply instantiate_gv__inhabited in H0. inv H0.
-  destruct (@mcast_is_total TD op t1 t2 x0) as [z J].
-  assert (J1:=@gv2gvs__inhabited z). inv J1.
-  exists x1. unfold Ensembles.In. exists x0. exists z.
-  split; auto. 
-Qed.
-
-Lemma instantiate_gv__mcast__helper2 : forall z xs
-  (H0 : instantiate_gv z xs),
-   instantiate_gv z
-     (fun gv2 : GenericValue =>
-      exists gv1 : GenericValue,
-        exists gv2' : GenericValue,
-          gv1 @ xs /\ ret gv1 = ret gv2' /\ gv2 @ $ gv2' $).
-Proof.
-  intros.
-  destruct z.
-    apply Extensionality_Ensembles in H0. subst. 
-    simpl. 
-    unfold Same_set, Included.
-    split; intros.
-      inv H. unfold Ensembles.In. exists nil. exists nil. simpl.
-      split. constructor. split; auto. constructor. 
-
-      inv H. destruct H0 as [A [J1 [J2 J3]]]. inv J1. inv J2. inv J3.
-      unfold Ensembles.In. constructor.
-
-    destruct p. 
-    destruct v; simpl in *.
-      destruct z.
-        inv H0.  
-        assert (J:=@gv2gvs__inhabited x). inv J.
-        exists x0. unfold Ensembles.In. exists x. exists x.
-        split; auto.
-             
-        apply Extensionality_Ensembles in H0. subst. 
-        unfold Same_set, Included.
-        split; intros.
-          inv H. unfold Ensembles.In. exists ((Vundef, m) :: p :: z). 
-          exists ((Vundef, m) :: p :: z). simpl.
-          split. constructor. split; auto. constructor. 
-
-          inv H. destruct H0 as [A [J1 [J2 J3]]]. inv J1. inv J2. inv J3.
-          constructor.
-   
-     apply Extensionality_Ensembles in H0. subst. 
-     unfold Same_set, Included.
-     split; intros.
-        inv H. unfold Ensembles.In. exists ((Vint wz i0, m) :: z). 
-        exists ((Vint wz i0, m) :: z). simpl.
-        split. constructor. split; auto. constructor. 
-
-        inv H. destruct H0 as [A [J1 [J2 J3]]]. inv J1. inv J2. inv J3.
-        constructor.
-
-     apply Extensionality_Ensembles in H0. subst. 
-     unfold Same_set, Included.
-     split; intros.
-        inv H. unfold Ensembles.In. exists ((Vfloat f, m) :: z). 
-        exists ((Vfloat f, m) :: z). simpl.
-        split. constructor. split; auto. constructor. 
-
-        inv H. destruct H0 as [A [J1 [J2 J3]]]. inv J1. inv J2. inv J3.
-        constructor.
-
-     apply Extensionality_Ensembles in H0. subst. 
-     unfold Same_set, Included.
-     split; intros.
-        inv H. unfold Ensembles.In. exists ((Vptr b i0, m) :: z). 
-        exists ((Vptr b i0, m) :: z). simpl.
-        split. constructor. split; auto. constructor. 
-
-        inv H. destruct H0 as [A [J1 [J2 J3]]]. inv J1. inv J2. inv J3.
-        constructor.
-
-     apply Extensionality_Ensembles in H0. subst. 
-     unfold Same_set, Included.
-     split; intros.
-        inv H. unfold Ensembles.In. exists ((Vinttoptr i0, m) :: z). 
-        exists ((Vinttoptr i0, m) :: z). simpl.
-        split. constructor. split; auto. constructor. 
-
-        inv H. destruct H0 as [A [J1 [J2 J3]]]. inv J1. inv J2. inv J3.
-        constructor.
-Qed.
-
-Lemma instantiate_gv__mcast : forall TD cop0 t1 t2 x z xs,
-  mcast TD cop0 t1 t2 x = Some z ->
-  instantiate_gv x xs ->
-  instantiate_gv z (lift_op1 (mcast TD cop0 t1 t2) xs).
-Proof.
-  intros. unfold lift_op1. 
-  unfold mcast, mbitcast in H.
-Opaque mcast. 
-  destruct cop0; try solve [inv H; simpl; 
-      eapply instantiate_gv__mcast__helper; eauto];
-    destruct t1; destruct t2; try solve [    
-      inv H; destruct f; 
-        try solve [simpl; eapply instantiate_gv__mcast__helper; eauto] |
-      inv H; destruct f0; 
-        try solve [simpl; eapply instantiate_gv__mcast__helper; eauto] |
-      inv H; try solve [simpl; eapply instantiate_gv__mcast__helper; eauto]
-    ].
-Transparent mcast. 
-    inv H; unfold mcast, mbitcast; apply instantiate_gv__mcast__helper2; auto.
-    inv H; unfold mcast, mbitcast; apply instantiate_gv__mcast__helper2; auto.
-    inv H; unfold mcast, mbitcast; apply instantiate_gv__mcast__helper2; auto.
-    inv H; unfold mcast, mbitcast; apply instantiate_gv__mcast__helper2; auto.
-    inv H; unfold mcast, mbitcast; apply instantiate_gv__mcast__helper2; auto.
-    inv H; unfold mcast, mbitcast; apply instantiate_gv__mcast__helper2; auto.
-    inv H; unfold mcast, mbitcast; apply instantiate_gv__mcast__helper2; auto.
-    inv H; unfold mcast, mbitcast; apply instantiate_gv__mcast__helper2; auto.
-    inv H; unfold mcast, mbitcast; apply instantiate_gv__mcast__helper2; auto.
-    inv H; unfold mcast, mbitcast; apply instantiate_gv__mcast__helper2; auto.
-Qed.    
 
 Lemma instantiate_locals__CAST : forall TD lc1 lc2 gl t1 v1 t2 gv2 castop0,
   instantiate_locals lc1 lc2 -> 
@@ -1591,7 +715,7 @@ Proof.
   unfold NDopsem.CAST.
   rewrite H1.
   exists (lift_op1 (mcast TD castop0 t1 t2) gvs1).
-  split; eauto using instantiate_gv__mcast.
+  split; eauto using instantiate_gv__lift_op1.
 Qed.
 
 Lemma mtrunc_is_total : forall TD top0 t1 t2 x, 
@@ -1604,134 +728,6 @@ Proof.
   destruct (floating_point_order f1 f0); eauto.
   destruct f1; eauto.
 Qed.
-
-Lemma instantiate_gv__mtrunc__helper : forall x xs TD op t1 t2
-  (H0 : instantiate_gv x xs),
-   Inhabited GenericValue
-     (fun gv2 : GenericValue =>
-      exists gv1 : GenericValue,
-        exists gv2' : GenericValue,
-            gv1 @ xs /\ mtrunc TD op t1 t2 gv1 = ret gv2' /\ gv2 @ $ gv2' $).
-Proof.
-  intros.
-  apply instantiate_gv__inhabited in H0. inv H0.
-  destruct (@mtrunc_is_total TD op t1 t2 x0) as [z J].
-  assert (J1:=@gv2gvs__inhabited z). inv J1.
-  exists x1. unfold Ensembles.In. exists x0. exists z.
-  split; auto. 
-Qed.
-
-Lemma instantiate_gv__mtrunc : forall TD top0 t1 t2 x z xs,
-  mtrunc TD top0 t1 t2 x = Some z ->
-  instantiate_gv x xs ->
-  instantiate_gv z (lift_op1 (mtrunc TD top0 t1 t2) xs).
-Proof.
-  intros. unfold lift_op1. 
-  unfold mtrunc in H.
-Opaque mtrunc. 
-  destruct x; try solve [
-    destruct t2; try solve [
-      inv H; simpl; eapply instantiate_gv__mtrunc__helper; eauto |
-      destruct f; try solve [inv H; simpl; 
-        eapply instantiate_gv__mtrunc__helper; eauto]
-    ]
-  ].
-  destruct p.
-  destruct x; try solve [
-    destruct t2; try solve [
-      inv H; simpl; eapply instantiate_gv__mtrunc__helper; eauto |
-      destruct f; try solve [inv H; simpl; 
-        eapply instantiate_gv__mtrunc__helper; eauto]
-    ]
-  ].
-  simpl in H.
-  destruct v; try solve [
-    destruct t2; try solve [
-      inv H; simpl; eapply instantiate_gv__mtrunc__helper; eauto |
-      destruct f; try solve [inv H; simpl; 
-        eapply instantiate_gv__mtrunc__helper; eauto]
-    ] |
-    destruct t1; destruct t2; try solve [
-      inv H; simpl; eapply instantiate_gv__mtrunc__helper; eauto |
-      destruct f0; try solve [inv H; simpl; 
-        eapply instantiate_gv__mtrunc__helper; eauto]
-    ]
-  ].
-
-    destruct t1; destruct t2; try solve [
-      inv H; simpl; eapply instantiate_gv__mtrunc__helper; eauto |
-      destruct f; try solve [inv H; simpl; 
-        eapply instantiate_gv__mtrunc__helper; eauto] |
-      destruct f0; try solve [inv H; simpl; 
-        eapply instantiate_gv__mtrunc__helper; eauto]
-    ]. 
-
-Transparent mtrunc. 
-      inv H.
-      unfold val2GV.
-      destruct (le_lt_dec wz s0); simpl.
-        eapply instantiate_gv__mtrunc__helper; eauto.
-
-        apply Extensionality_Ensembles in H0. subst. 
-        unfold Same_set, Included.
-        split; intros.
-          inv H. unfold Ensembles.In.
-          exists ((Vint wz i0, m) :: nil). 
-          unfold mtrunc. simpl.
-          destruct (le_lt_dec wz s0); simpl.
-            contradict l1. omega.
-            unfold val2GV.
-            exists ((Vint s0 (Int.repr s0 (Int.unsigned wz i0)), AST.Mint s0) :: nil).                    
-            simpl. split. constructor. split; auto. constructor.
-
-          inv H. destruct H0 as [gv2' [J1 [J2 J3]]].
-          inv J1. unfold mtrunc in J2. simpl in J2. inv J2.
-          destruct (le_lt_dec wz s0); simpl.
-            contradict l1. omega.
-            unfold val2GV in J3. inv J3.
-            constructor.
-
-    destruct t1; destruct t2; try solve [
-      inv H; simpl; eapply instantiate_gv__mtrunc__helper; eauto |
-      destruct f0; try solve [inv H; simpl; 
-        eapply instantiate_gv__mtrunc__helper; eauto]
-    ]. 
-
-      remember (floating_point_order f1 f0) as R.
-      destruct R; destruct f1; try solve [
-        inv H; simpl; eapply instantiate_gv__mtrunc__helper; eauto].
-      apply Extensionality_Ensembles in H0. subst. inv H.
-      unfold val2GV. simpl.
-      unfold Same_set, Included.
-      split; intros.
-        inv H. unfold Ensembles.In.
-        exists ((Vfloat f, m) :: nil). 
-        unfold mtrunc. simpl. rewrite <- HeqR.
-        unfold val2GV.
-        exists ((Vfloat f, AST.Mfloat32) :: nil).                    
-        simpl. split. constructor. split; auto. constructor.
-
-        inv H. destruct H0 as [gv2' [J1 [J2 J3]]].
-        inv J1. unfold mtrunc in J2. simpl in J2. 
-        rewrite <- HeqR in J2. inv J2. inv J3.
-        constructor.
-
-     inv H.
-     apply Extensionality_Ensembles in H0. subst. simpl.
-     unfold Same_set, Included.
-     split; intros.
-       inv H. unfold Ensembles.In.
-       exists ((Vfloat f, m) :: nil). 
-       unfold mtrunc. simpl. rewrite <- HeqR.
-       unfold val2GV.
-       exists ((Vfloat f, AST.Mfloat64) :: nil).                    
-       simpl. split. constructor. split; auto. constructor.
-
-       inv H. destruct H0 as [gv2' [J1 [J2 J3]]].
-       inv J1. unfold mtrunc in J2. simpl in J2. 
-       rewrite <- HeqR in J2. inv J2. inv J3.
-       constructor.     
-Qed.    
 
 Lemma instantiate_locals__TRUNC : forall TD lc1 lc2 gl t1 v1 t2 gv2 top0,
   instantiate_locals lc1 lc2 -> 
@@ -1747,7 +743,7 @@ Proof.
   unfold NDopsem.TRUNC.
   rewrite H1.
   exists (lift_op1 (mtrunc TD top0 t1 t2) gvs1).
-  split; eauto using instantiate_gv__mtrunc.
+  split; eauto using instantiate_gv__lift_op1.
 Qed.
 
 Lemma mext_is_total : forall TD eop0 t1 t2 x, 
@@ -1765,107 +761,6 @@ Proof.
     try solve [destruct (floating_point_order f f0); eauto | eauto].
 Qed.
 
-Lemma instantiate_gv__mext__helper : forall x xs TD op t1 t2
-  (H0 : instantiate_gv x xs),
-   Inhabited GenericValue
-     (fun gv2 : GenericValue =>
-      exists gv1 : GenericValue,
-        exists gv2' : GenericValue,
-            gv1 @ xs /\ mext TD op t1 t2 gv1 = ret gv2' /\ gv2 @ $ gv2' $).
-Proof.
-  intros.
-  apply instantiate_gv__inhabited in H0. inv H0.
-  destruct (@mext_is_total TD op t1 t2 x0) as [z J].
-  assert (J1:=@gv2gvs__inhabited z). inv J1.
-  exists x1. unfold Ensembles.In. exists x0. exists z.
-  split; auto. 
-Qed.
-
-Lemma instantiate_gv__mext : forall TD eop0 t1 t2 x z xs,
-  mext TD eop0 t1 t2 x = Some z ->
-  instantiate_gv x xs ->
-  instantiate_gv z (lift_op1 (mext TD eop0 t1 t2) xs).
-Proof.
-  intros. unfold lift_op1. 
-  unfold mext in H.
-Opaque mext. 
-  destruct t1; destruct t2; try solve [
-    inv H; simpl; eapply instantiate_gv__mext__helper; eauto |
-    inv H; destruct f; simpl; eapply instantiate_gv__mext__helper; eauto
-  ].
-
-  destruct x; try solve 
-    [inv H; simpl; eapply instantiate_gv__mext__helper; eauto].
-  destruct p.
-  destruct x; try solve 
-    [inv H; simpl; eapply instantiate_gv__mext__helper; eauto].
-  destruct v; try solve 
-    [inv H; simpl; eapply instantiate_gv__mext__helper; eauto].
-  destruct eop0; try solve 
-    [inv H; simpl; eapply instantiate_gv__mext__helper; eauto].
-
-Transparent mext. 
-    inv H.
-    apply Extensionality_Ensembles in H0. subst. simpl.
-    unfold Same_set, Included.
-    split; intros.
-      inv H. unfold Ensembles.In. 
-      exists ((Vint wz i0, m) :: nil).
-      exists (val2GV TD (Vint wz (Int.zero_ext wz (Size.to_Z s0) i0))
-          (AST.Mint (Size.to_nat s0 - 1))).  
-      split. constructor.
-      unfold mext. simpl. split; auto. constructor.
-
-      inv H. destruct H0 as [gv2' [J1 [J2 J3]]].
-      inv J1. unfold mext in J2. simpl in J2. inv J2. inv J3.
-      constructor.
-
-Transparent mext. 
-    inv H.
-    apply Extensionality_Ensembles in H0. subst. simpl.
-    unfold Same_set, Included.
-    split; intros.
-      inv H. unfold Ensembles.In. 
-      exists ((Vint wz i0, m) :: nil).
-      exists (val2GV TD (Vint wz (Int.sign_ext wz (Size.to_Z s0) i0))
-          (AST.Mint (Size.to_nat s0 - 1))).  
-      split. constructor.
-      unfold mext. simpl. split; auto. constructor.
-
-      inv H. destruct H0 as [gv2' [J1 [J2 J3]]].
-      inv J1. unfold mext in J2. simpl in J2. inv J2. inv J3.
-      constructor.
-
-  remember (floating_point_order f f0) as R.
-  destruct R; simpl; try solve [
-    destruct f0; inv H; simpl; eapply instantiate_gv__mext__helper; eauto
-  ].
-  destruct x; try solve 
-    [inv H; destruct f0; simpl; eapply instantiate_gv__mext__helper; eauto].
-  destruct p.
-  destruct x; try solve 
-    [inv H; destruct f0; simpl; eapply instantiate_gv__mext__helper; eauto].
-  destruct v; try solve 
-    [inv H; destruct f0; simpl; eapply instantiate_gv__mext__helper; eauto].
-  destruct eop0; try solve 
-    [inv H; destruct f0; simpl; eapply instantiate_gv__mext__helper; eauto].
-
-Transparent mext. 
-    inv H.
-    apply Extensionality_Ensembles in H0. subst. simpl.
-    unfold Same_set, Included.
-    split; intros.
-      inv H. unfold Ensembles.In. 
-      exists ((Vfloat f1, m) :: nil).
-      exists ((Vfloat f1, m) :: nil).
-      split. constructor.
-      unfold mext. simpl. rewrite <- HeqR. split; auto. constructor.
-
-      inv H. destruct H0 as [gv2' [J1 [J2 J3]]].
-      inv J1. unfold mext in J2. rewrite <- HeqR in J2. inv J2. inv J3.
-      constructor.
-Qed.    
-
 Lemma instantiate_locals__EXT : forall TD lc1 lc2 gl t1 v1 t2 gv2 top0,
   instantiate_locals lc1 lc2 -> 
   EXT TD lc1 gl top0 t1 v1 t2 = Some gv2 ->
@@ -1880,7 +775,7 @@ Proof.
   unfold NDopsem.EXT.
   rewrite H1.
   exists (lift_op1 (mext TD top0 t1 t2) gvs1).
-  split; eauto using instantiate_gv__mext.
+  split; eauto using instantiate_gv__lift_op1.
 Qed.
 
 Lemma lookupFdefViaGV_inversion : forall TD Ps gl lc fs fv f,
@@ -2096,89 +991,30 @@ Proof.
     apply instantiate_locals__updateAddAL; auto using instantiate_gv__gv2gvs.
 Qed.
 
-Definition undef_state St : Prop :=
-  match St with 
-  | {| CurTargetData := TD;
-       ECS := {| CurCmds := nil;
-                 Terminator := insn_br _ Cond _ _;
-                 Locals := lc |} :: _;
-       Globals := gl |} =>
-     match getOperandValue TD Cond lc gl with
-     | ret c => ~ defined_gv c 
-     | _ => False
-     end
-  | {| CurTargetData := TD;
-       ECS := {| CurCmds := insn_store _ _ v _ _::_;
-                 Locals := lc |} :: _;
-       Globals := gl |} =>
-     match getOperandValue TD v lc gl with
-     | ret gv => ~ defined_gv gv 
-     | _ => False
-     end
-  | {| CurTargetData := TD;
-       ECS := {| CurCmds := insn_call _ _ _ _ fv lp::_;
-                 Locals := lc |} :: _;
-       Globals := gl |} =>
-     match getOperandValue TD fv lc gl, params2GVs TD lp lc gl with
-     | ret gv, ret gvs => ~ defined_gv gv \/ ~ defined_gvs gvs
-     | _, _ => False
-     end
-  |  {| CurTargetData := TD;
-       ECS := {| CurCmds := insn_select _ v _ _ _::_;
-                 Locals := lc |} :: _;
-       Globals := gl |} =>
-     match getOperandValue TD v lc gl with
-     | ret gv => ~ defined_gv gv 
-     | _ => False
-     end
-  |  {| CurTargetData := TD;
-       ECS := {| CurCmds := insn_extractvalue _ _ v _::_;
-                 Locals := lc |} :: _;
-       Globals := gl |} =>
-     match getOperandValue TD v lc gl with
-     | ret gv => ~ defined_gv gv 
-     | _ => False
-     end
-  |  {| CurTargetData := TD;
-       ECS := {| CurCmds := insn_insertvalue _ _ v1 _ v2 _ ::_;
-                 Locals := lc |} :: _;
-       Globals := gl |} =>
-     match getOperandValue TD v1 lc gl, getOperandValue TD v2 lc gl with
-     | ret gv1, ret gv2 => ~ defined_gv gv1 \/ ~ defined_gv gv2  
-     | _, _ => False
-     end
-  | _ => False
-  end.
-
 Lemma instantiate_dsInsn : forall st1 st2 st1' tr,
   instantiate_State st1 st2 ->
   LLVMopsem.dsInsn st1 st1' tr ->
-  (exists st2', NDopsem.nsInsn st2 st2' tr /\ instantiate_State st1' st2') \/
-  undef_state st1.
+  (exists st2', NDopsem.nsInsn st2 st2' tr /\ instantiate_State st1' st2').
 Proof.
   intros st1 st2 st1' tr Hsim Hop.  
   (dsInsn_cases (induction Hop) Case).
 Case "dsReturn". simpl_nd_llvmds. 
   eapply instantiate_locals__returnUpdateLocals in H1; eauto.
   destruct H1 as [lc2'' [H1 H2]].
-  left. exists (NDopsem.mkState S' TD' Ps' 
+  exists (NDopsem.mkState S' TD' Ps' 
     ((NDopsem.mkEC f2' b2' cs' tmn2' lc2'' als2')::ECs') gl' fs' Mem').
   split; eauto.
     repeat (split; auto).
 Case "dsReturnVoid". simpl_nd_llvmds. 
-  left. exists (NDopsem.mkState S' TD' Ps' 
+  exists (NDopsem.mkState S' TD' Ps' 
     ((NDopsem.mkEC f2' b2' cs' tmn2' lc2' als2')::ECs') gl' fs' Mem').
   split; eauto.
     repeat (split; auto).
 Case "dsBranch". simpl_nd_llvmds. 
-  simpl. rewrite H.
-  destruct (@defined_gv_dec c) as [Hdet | Hndet]; auto.
-  left.
   eapply instantiate_locals__switchToNewBasicBlock in H1; eauto.
   eapply instantiate_locals__getOperandValue in H; eauto.
   destruct H as [gvs2 [J1 J2]].
   destruct H1 as [lc2' [J3 J4]].
-  apply defined_gv__instantiate_gv in J2; auto.   
   exists (NDopsem.mkState S' TD' Ps' 
     ((NDopsem.mkEC f1' (block_intro l' ps' cs' tmn') cs' tmn' lc2' als1')
       ::ECs') gl' fs' M').
@@ -2186,7 +1022,7 @@ Case "dsBranch". simpl_nd_llvmds.
     repeat (split; auto).
 Case "dsBranch_uncond". simpl_nd_llvmds. 
   eapply instantiate_locals__switchToNewBasicBlock in H0; eauto.
-  destruct H0 as [lc2' [J1 J2]]. left.
+  destruct H0 as [lc2' [J1 J2]]. 
   exists (NDopsem.mkState S' TD' Ps' 
     ((NDopsem.mkEC f1' (block_intro l' ps' cs' tmn') cs' tmn' lc2' als1')
       ::ECs') gl' fs' M').
@@ -2194,7 +1030,7 @@ Case "dsBranch_uncond". simpl_nd_llvmds.
     repeat (split; auto).
 Case "dsBop". simpl_nd_llvmds. 
   eapply instantiate_locals__BOP in H; eauto.
-  destruct H as [gvs3' [J1 J2]]. left.
+  destruct H as [gvs3' [J1 J2]].
   exists (NDopsem.mkState S' TD' Ps' 
     ((NDopsem.mkEC f1' b1' cs tmn1' (updateAddAL _ lc1' id0 gvs3') als1')
       ::ECs') gl' fs' M').
@@ -2202,16 +1038,13 @@ Case "dsBop". simpl_nd_llvmds.
     repeat (split; auto using instantiate_locals__updateAddAL).
 Case "dsFBop". simpl_nd_llvmds. 
   eapply instantiate_locals__FBOP in H; eauto.
-  destruct H as [gvs3' [J1 J2]]. left.
+  destruct H as [gvs3' [J1 J2]]. 
   exists (NDopsem.mkState S' TD' Ps' 
     ((NDopsem.mkEC f1' b1' cs tmn1' (updateAddAL _ lc1' id0 gvs3') als1')
       ::ECs') gl' fs' M').
   split; eauto.
     repeat (split; auto using instantiate_locals__updateAddAL).
 Case "dsExtractValue". simpl_nd_llvmds. 
-  simpl. rewrite H.
-  destruct (@defined_gv_dec gv) as [Hdet | Hndet]; auto.
-  left.
   eapply instantiate_locals__getOperandValue in H; eauto.
   destruct H as [gvs [J1 J2]].
   eapply instantiate_locals__extractGenericValue in H0; eauto.
@@ -2222,10 +1055,6 @@ Case "dsExtractValue". simpl_nd_llvmds.
   split; eauto.
     repeat (split; auto using instantiate_locals__updateAddAL).
 Case "dsInsertValue". simpl_nd_llvmds. 
-  simpl. rewrite H. rewrite H0.
-  destruct (@defined_gv_dec gv) as [Hdet | Hndet]; auto.
-  destruct (@defined_gv_dec gv') as [Hdet' | Hndet']; auto.
-  left.
   eapply instantiate_locals__getOperandValue in H; eauto.
   destruct H as [gvs [J1 J2]].
   eapply instantiate_locals__getOperandValue in H0; eauto.
@@ -2238,12 +1067,8 @@ Case "dsInsertValue". simpl_nd_llvmds.
   split; eauto.
     repeat (split; auto using instantiate_locals__updateAddAL).
 Case "dsMalloc". simpl_nd_llvmds. 
-  assert (J:=H1).
-  apply malloc__defined_gv in J.
-  left.
   eapply instantiate_locals__getOperandValue in H0; eauto.
   destruct H0 as [gns [J1 J2]].
-  apply defined_gv__instantiate_gv in J2; auto.   
   exists (NDopsem.mkState S' TD' Ps' 
     ((NDopsem.mkEC f1' b1' cs tmn1' 
       (updateAddAL _ lc1' id0 ($ (blk2GV TD' mb) $)) 
@@ -2252,24 +1077,16 @@ Case "dsMalloc". simpl_nd_llvmds.
     repeat (split; auto using instantiate_locals__updateAddAL, 
                               instantiate_gv__gv2gvs).
 Case "dsFree". simpl_nd_llvmds. 
-  assert (J:=H0).
-  apply free__defined_gv in J.
-  left.
   eapply instantiate_locals__getOperandValue in H; eauto.
   destruct H as [gvs [J1 J2]].
-  apply defined_gv__instantiate_gv in J2; auto.   
   exists (NDopsem.mkState S' TD' Ps' 
     ((NDopsem.mkEC f1' b1' cs tmn1' lc1'
     als1')::ECs') gl' fs' Mem').
   split; eauto. 
     repeat (split; auto).
 Case "dsAlloca". simpl_nd_llvmds. 
-  assert (J:=H1).
-  apply malloc__defined_gv in J.
-  left.
   eapply instantiate_locals__getOperandValue in H0; eauto.
   destruct H0 as [gns [J1 J2]].
-  apply defined_gv__instantiate_gv in J2; auto.   
   exists (NDopsem.mkState S' TD' Ps' 
     ((NDopsem.mkEC f1' b1' cs tmn1' 
       (updateAddAL _ lc1' id0 ($ (blk2GV TD' mb) $)) 
@@ -2278,12 +1095,8 @@ Case "dsAlloca". simpl_nd_llvmds.
     repeat (split; auto using instantiate_locals__updateAddAL, 
                               instantiate_gv__gv2gvs).
 Case "dsLoad". simpl_nd_llvmds.
-  assert (J:=H0).
-  apply mload__defined_gv in J.
-  left.
   eapply instantiate_locals__getOperandValue in H; eauto.
   destruct H as [gvs2 [J1 J2]].
-  apply defined_gv__instantiate_gv in J2; auto.   
   exists (NDopsem.mkState S' TD' Ps' 
     ((NDopsem.mkEC f1' b1' cs tmn1' (updateAddAL _ lc1' id0 ($ gv $))
     als1')::ECs') gl' fs' M').
@@ -2291,17 +1104,10 @@ Case "dsLoad". simpl_nd_llvmds.
     repeat (split; auto using instantiate_locals__updateAddAL, 
                               instantiate_gv__gv2gvs).
 Case "dsStore". simpl_nd_llvmds.
-  assert (J:=H1).
-  apply mstore__defined_gv in J.
-  simpl. rewrite H.
-  destruct (@defined_gv_dec gv1) as [Hdet | Hndet]; auto.
-  left.
   eapply instantiate_locals__getOperandValue in H; eauto.
   destruct H as [gvs2 [J1 J2]].
-  apply defined_gv__instantiate_gv in J2; auto.   
   eapply instantiate_locals__getOperandValue in H0; eauto.
   destruct H0 as [mps2 [J3 J4]].
-  apply defined_gv__instantiate_gv in J4; auto.   
   exists (NDopsem.mkState S' TD' Ps' 
     ((NDopsem.mkEC f1' b1' cs tmn1' lc1' als1')::ECs') gl' fs' Mem').
   split; eauto. 
@@ -2312,13 +1118,13 @@ Case "dsGEP". simpl_nd_llvmds.
   eapply instantiate_locals__values2GVs in H0; eauto.
   destruct H0 as [vidxss [J3 J4]].
   eapply instantiate_locals__GEP in H1; eauto.
-  destruct H1 as [mps2' [J5 J6]]. left.
+  destruct H1 as [mps2' [J5 J6]].
   exists (NDopsem.mkState S' TD' Ps' 
     ((NDopsem.mkEC f1' b1' cs tmn1' (updateAddAL _ lc1' id0 mps2') als1')
       ::ECs') gl' fs' M').
   split; eauto.
     repeat (split; auto using instantiate_locals__updateAddAL).
-Case "dsTrunc". simpl_nd_llvmds. left.
+Case "dsTrunc". simpl_nd_llvmds.
   eapply instantiate_locals__TRUNC in H; eauto.
   destruct H as [gvs2' [J1 J2]].
   exists (NDopsem.mkState S' TD' Ps' 
@@ -2326,7 +1132,7 @@ Case "dsTrunc". simpl_nd_llvmds. left.
       ::ECs') gl' fs' M').
   split; eauto.
     repeat (split; auto using instantiate_locals__updateAddAL).
-Case "dsExt". simpl_nd_llvmds. left.
+Case "dsExt". simpl_nd_llvmds. 
   eapply instantiate_locals__EXT in H; eauto.
   destruct H as [gvs2' [J1 J2]].
   exists (NDopsem.mkState S' TD' Ps' 
@@ -2334,7 +1140,7 @@ Case "dsExt". simpl_nd_llvmds. left.
       ::ECs') gl' fs' M').
   split; eauto.
     repeat (split; auto using instantiate_locals__updateAddAL).
-Case "dsCast". simpl_nd_llvmds. left.
+Case "dsCast". simpl_nd_llvmds. 
   eapply instantiate_locals__CAST in H; eauto.
   destruct H as [gvs2' [J1 J2]].
   exists (NDopsem.mkState S' TD' Ps' 
@@ -2344,7 +1150,7 @@ Case "dsCast". simpl_nd_llvmds. left.
     repeat (split; auto using instantiate_locals__updateAddAL).
 Case "dsIcmp". simpl_nd_llvmds. 
   eapply instantiate_locals__ICMP in H; eauto.
-  destruct H as [gvs3' [J1 J2]]. left.
+  destruct H as [gvs3' [J1 J2]].
   exists (NDopsem.mkState S' TD' Ps' 
     ((NDopsem.mkEC f1' b1' cs tmn1' (updateAddAL _ lc1' id0 gvs3') als1')
       ::ECs') gl' fs' M').
@@ -2352,19 +1158,15 @@ Case "dsIcmp". simpl_nd_llvmds.
     repeat (split; auto using instantiate_locals__updateAddAL).
 Case "dsFcmp". simpl_nd_llvmds. 
   eapply instantiate_locals__FCMP in H; eauto.
-  destruct H as [gvs3' [J1 J2]]. left.
+  destruct H as [gvs3' [J1 J2]]. 
   exists (NDopsem.mkState S' TD' Ps' 
     ((NDopsem.mkEC f1' b1' cs tmn1' (updateAddAL _ lc1' id0 gvs3') als1')
       ::ECs') gl' fs' M').
   split; eauto.
     repeat (split; auto using instantiate_locals__updateAddAL).
 Case "dsSelect". simpl_nd_llvmds. 
-  simpl. rewrite H.
-  destruct (@defined_gv_dec c) as [Hdet | Hndet]; auto.
-  left.
   eapply instantiate_locals__getOperandValue in H; eauto.
   destruct H as [gvs0' [J1 J2]].
-  apply defined_gv__instantiate_gv in J2; auto.   
   eapply instantiate_locals__getOperandValue in H0; eauto.
   destruct H0 as [gvs1' [J3 J4]].
   eapply instantiate_locals__getOperandValue in H1; eauto.
@@ -2380,12 +1182,8 @@ Case "dsSelect". simpl_nd_llvmds.
 Case "dsCall". simpl_nd_llvmds. 
   apply lookupFdefViaGV_inversion in H.
   destruct H as [fptr [fn [J1 [J2 J3]]]].
-  simpl. rewrite J1. rewrite H1.
-  destruct (@defined_gv_dec fptr) as [Hdet | Hndet]; auto.
-  left.
   eapply instantiate_locals__getOperandValue in J1; eauto.
   destruct J1 as [gvs2 [J11 J12]].
-  apply defined_gv__instantiate_gv in J12; auto.   
   eapply instantiate_locals__params2GVs in H1; eauto.
   destruct H1 as [gvss2 [H11 H12]].
   exists (NDopsem.mkState S' TD' Ps' 
@@ -2403,16 +1201,10 @@ Case "dsCall". simpl_nd_llvmds.
 Case "dsExCall". simpl_nd_llvmds. 
   apply lookupExFdecViaGV_inversion in H.
   destruct H as [fptr [fn [J1 [J2 [J3 J4]]]]].
-  simpl. rewrite J1. rewrite H0.
-  destruct (@defined_gv_dec fptr) as [Hdet | Hndet]; auto.
-  destruct (@defined_gvs_dec gvs) as [Hdet' | Hndet']; auto.
-  left.
   eapply instantiate_locals__getOperandValue in J1; eauto.
   destruct J1 as [gvs2 [J11 J12]].
-  apply defined_gv__instantiate_gv in J12; auto.   
   eapply instantiate_locals__params2GVs in H0; eauto.
   destruct H0 as [gvss2 [H11 H12]].
-  apply defined_gvs__instantiate_gvs in H12; auto.
   eapply instantiate_locals__exCallUpdateLocals in H2; eauto.
   destruct H2 as [lc2' [H21 H22]].
   exists (NDopsem.mkState S' TD' Ps' 
